

$$\textcircled{1} \int (\sqrt[3]{x^2} + \frac{1}{\sqrt{x}}) dx$$

$$\sqrt[3]{x^2} = x^{2/3} \quad \text{= suku pertama}$$

$$\frac{1}{\sqrt{x}} = \frac{1}{x^{1/2}} = x^{-1/2} \quad \text{= suku kedua}$$

$$\int (x^{2/3} + x^{-1/2}) dx$$

$$\int x^{2/3} dx$$

$$\int x^{2/3} dx = \frac{1}{\frac{5}{3}} x^{5/3} = \frac{3}{5} x^{5/3}$$

$$\int x^{-1/2} dx$$

$$\int x^{-1/2} dx = \frac{1}{1/2} x^{1/2} = 2x^{1/2}$$

$$\int (x^{2/3} + x^{-1/2}) dx = \frac{3}{5} x^{5/3} + 2x^{1/2} + C$$

$$x^{5/3} = x^{1 2/3} \cdot x^{1/3} = x \sqrt[3]{x^2}$$

$$x^{1/2} = \sqrt{x}$$

$$= \int (\sqrt[3]{x^2} + \frac{1}{\sqrt{x}}) dx = \frac{3}{5} \sqrt[3]{x^5} + 2\sqrt{x} + C$$

$$② \int (\sqrt{2x+1})^3 \sqrt{2} dx$$

$$= \int ((2x+1)^{1/2})^3 \sqrt{2} dx$$

$$\int (2x+1)^{3/2} \sqrt{2} dx$$

$$\sqrt{2} \int (2x+1)^{3/2} dx$$

$$\sqrt{2} \int (u)^{3/2} \left(\frac{1}{2} du \right)$$

$$\frac{\sqrt{2}}{2} \int u^{3/2} du$$

$$\frac{\sqrt{2}}{2} \left[\frac{1}{5/2} u^{5/2} \right] + C$$

$$\frac{\sqrt{2}}{2} \left[\frac{2}{5} u^{5/2} \right] + C$$

$$\frac{\sqrt{2}}{2} \cdot \frac{2}{5} = \frac{\sqrt{2}}{5} u^{5/2} + C$$

$$\frac{\sqrt{2}}{5} \sqrt{(2x+1)^5} + C$$

$$\int (\sqrt{2x+1})^3 \sqrt{2} dx = \frac{\sqrt{2}}{5} (2x+1)^{5/2} + C$$

$$(3) \int \frac{2v}{\sqrt{2v^2 + 5}} dv$$

$$\int 2v (2v^2 + 5)^{-1/2} dv$$

$$u = 2v^2 + 5$$

$$du = \frac{d}{dv} (2v^2 + 5) dv \Rightarrow du = 4v dv$$

$$\frac{1}{2} du = 2v dv$$

$$\int (u)^{-1/2} \left(\frac{1}{2} du\right)$$

$$\frac{1}{2} \int u^{-1/2} du$$

$$\frac{1}{2} \left[\frac{1}{1/2} u^{1/2} \right] + C$$

$$\frac{1}{2} \left[2u^{1/2} \right] + C$$

$$\frac{1}{2} \cdot 2 = 1 \quad u^{1/2} + C$$

$$(2v^2 + 5)^{1/2} + C$$

$$\sqrt{2v^2 + 5} + C$$

$$\int \frac{2v}{\sqrt{2v^2 + 5}} dv = \sqrt{2v^2 + 5} + C$$

$$1) \int_0^{30^\circ} (\cos x (1 - \sin x)) dx$$

$$\int_0^{\pi/6} (\cos x - \cos x \sin x) dx$$

$$\int (\cos x) dx - \int (\cos x \sin x) dx$$

$$\int \cos x dx = \sin x$$

$$\int u du = \frac{1}{2} u^2$$

$$\int \cos x \sin x dx = \frac{1}{2} \sin^2 x$$

$$\int (\cos x - \cos x \sin x) dx = \sin x - \frac{1}{2} \sin^2 x + C$$